Specify Create API

src/proof/well_formed.v
@@ -12,15 +12,37 @@ Context `{hG: !heapGS Σ} {go_ctx: GoContext}.
 Definition object_meta_well_formed (m: v1.ObjectMeta.t) : iProp Σ :=
   "uid_well_formed" ∷ ⌜ m.(v1.ObjectMeta.UID') ≠ "_ORPHAN_POD"%go ⌝.
 
-Definition pod_well_formed (pod: v1.Pod.t) : iProp Σ :=
-  "pod_metadata_well_formed" ∷ object_meta_well_formed pod.(v1.Pod.ObjectMeta').
+Axiom pod_spec_well_formed: v1.PodSpec.t → iProp Σ.
 
-Axiom pod_well_formed_for_creation: v1.Pod.t → iProp Σ.
+Axiom pod_status_well_formed: v1.PodStatus.t → iProp Σ.
+
+Definition pod_well_formed (pod: v1.Pod.t) : iProp Σ :=
+  "pod_metadata_well_formed" ∷ object_meta_well_formed pod.(v1.Pod.ObjectMeta') ∗
+  "pod_spec_well_formed" ∷ pod_spec_well_formed pod.(v1.Pod.Spec') ∗
+  "pod_status_well_formed" ∷ pod_status_well_formed pod.(v1.Pod.Status').
 
 Definition pod_nn_well_formed (pod: v1.Pod.t) (namespace name: go_string) : iProp Σ :=
   "%namespace_match" ∷ ⌜ pod.(v1.Pod.ObjectMeta').(v1.ObjectMeta.Namespace') = namespace ⌝ ∗
   "%name_match" ∷ ⌜ pod.(v1.Pod.ObjectMeta').(v1.ObjectMeta.Name') = name ⌝ ∗
   "pod_well_formed" ∷ pod_well_formed pod.
+
+Definition object_meta_to_create_well_formed (m: v1.ObjectMeta.t) : iProp Σ :=
+  "generatename_not_empty_if_name_empty" ∷ ⌜ m.(v1.ObjectMeta.Name') = ""%go → m.(v1.ObjectMeta.GenerateName') ≠ ""%go ⌝.
+
+Axiom pod_spec_to_create_well_formed: v1.PodSpec.t → iProp Σ.
+
+Axiom pod_status_to_create_well_formed: v1.PodStatus.t → iProp Σ.
+
+Definition pod_to_create_well_formed (pod: v1.Pod.t) : iProp Σ :=
+  "pod_metadata_to_create_well_formed" ∷ object_meta_to_create_well_formed pod.(v1.Pod.ObjectMeta') ∗
+  "pod_spec_to_create_well_formed" ∷ pod_spec_to_create_well_formed pod.(v1.Pod.Spec') ∗
+  "pod_status_to_create_well_formed" ∷ pod_status_to_create_well_formed pod.(v1.Pod.Status').
+
+Definition pod_to_create_nn_well_formed (pod: v1.Pod.t) (namespace name: go_string) : iProp Σ :=
+  "%namespace_match" ∷ ⌜ pod.(v1.Pod.ObjectMeta').(v1.ObjectMeta.Namespace') = namespace ⌝ ∗
+  "%name_match" ∷ ⌜ pod.(v1.Pod.ObjectMeta').(v1.ObjectMeta.Name') = name ⌝ ∗
+  "pod_to_create_well_formed" ∷ pod_to_create_well_formed pod.
+
 
 Definition replicaset_well_formed (rs: v1.ReplicaSet.t) : iProp Σ :=
   object_meta_well_formed rs.(v1.ReplicaSet.ObjectMeta') ∗
