src/proof/apimodel.v
@@ -285,7 +285,37 @@ Lemma wp_ByIndex_pod_ptsto_mut kind index_name indexed_value
 Proof.
 Admitted.
 
-Lemma wp_PodCreate_without_name namespace to_create_pod_ptr to_create_pod
+Lemma wp_objCreate_pod_without_name_ptsto_mut kind namespace obj
+  to_create_pod_ptr to_create_pod γ_state γ_children γ_fresh_keys parent_key owned_parent owned_child_keys:
+  {{{ is_pkg_init apimodel ∗
+      "#inv" ∷ is_kubernetes_state γ_state γ_children γ_fresh_keys ∗
+      "own_parent" ∷ parent_key [[ γ_state ]]↦ owned_parent ∗
+      "own_child_keys" ∷ parent_key [[ γ_children ]]↦ owned_child_keys ∗
+      "%namespace_valid" ∷ ⌜ namespace = parent_key.(KKey.Namespace') ⌝ ∗
+      "%kind" ∷ ⌜ kind = "Pod"%go ⌝ ∗
+      "%interface_is_rs_ptr" ∷ ⌜ obj = interface.mk (ptrT.id v1.Pod.id) #to_create_pod_ptr ⌝ ∗
+      "to_create_pod_ptr" ∷ to_create_pod_ptr ↦ to_create_pod ∗
+      "to_create_pod_is_child" ∷ has_controller_parent_of to_create_pod.(v1.Pod.ObjectMeta').(v1.ObjectMeta.OwnerReferences') (extract_kobject_metadata owned_parent).(v1.ObjectMeta.UID') ∗
+      "well_formed_for_creation" ∷ pod_to_create_nn_well_formed to_create_pod namespace ""%go
+  }}}
+    @! apimodel.PodCreate #namespace #to_create_pod_ptr
+  {{{ created_obj (err: error.t) created_pod_ptr created_pod new_key, RET (#created_obj, #err);
+      ⌜ err = interface.nil ⌝ ∗
+      ⌜ created_obj = interface.mk (ptrT.id v1.Pod.id) #created_pod_ptr ⌝ ∗
+      created_pod_ptr ↦ created_pod ∗
+      pod_well_formed created_pod ∗
+      ⌜ new_key = extract_pod_key created_pod ⌝ ∗
+      ⌜ new_key ∉ owned_child_keys ⌝ ∗
+      new_key [[ γ_state ]]↦ (KObject.Pod created_pod) ∗
+      parent_key [[ γ_state ]]↦ owned_parent ∗
+      parent_key [[ γ_children ]]↦ (owned_child_keys ∪ {[new_key]})
+      (* TODO: specify that created_pod shares some contents with to_create_pod *)
+  }}}.
+Proof.
+  wp_start as "H". iNamed "H".
+Admitted.
+
+Lemma wp_PodCreate_without_name_ptsto_mut namespace to_create_pod_ptr to_create_pod
   γ_state γ_children γ_fresh_keys parent_key owned_parent owned_child_keys:
   {{{ is_pkg_init apimodel ∗
       "#inv" ∷ is_kubernetes_state γ_state γ_children γ_fresh_keys ∗
@@ -294,11 +324,9 @@ Lemma wp_PodCreate_without_name namespace to_create_pod_ptr to_create_pod
       "%namespace_valid" ∷ ⌜ namespace = parent_key.(KKey.Namespace') ⌝ ∗
       "to_create_pod_ptr" ∷ to_create_pod_ptr ↦ to_create_pod ∗
       "parent_uid" ∷ has_controller_parent_of to_create_pod.(v1.Pod.ObjectMeta').(v1.ObjectMeta.OwnerReferences') (extract_kobject_metadata owned_parent).(v1.ObjectMeta.UID') ∗
-      "%no_name" ∷ ⌜ to_create_pod.(v1.Pod.ObjectMeta').(v1.ObjectMeta.Name') = ""%go ⌝ ∗
-      "%generate_name" ∷ ⌜ to_create_pod.(v1.Pod.ObjectMeta').(v1.ObjectMeta.Name') ≠ ""%go⌝ ∗
-      "well_formed_for_creation" ∷ pod_well_formed_for_creation to_create_pod
+      "well_formed_for_creation" ∷ pod_to_create_nn_well_formed to_create_pod namespace ""%go
   }}}
-    @! apimodel.objCreate #namespace #to_create_pod_ptr
+    @! apimodel.PodCreate #namespace #to_create_pod_ptr
   {{{ created_pod_ptr (err: error.t) created_pod new_key, RET (#created_pod_ptr, #err);
       ⌜ err = interface.nil ⌝ ∗
       created_pod_ptr ↦ created_pod ∗
@@ -311,6 +339,7 @@ Lemma wp_PodCreate_without_name namespace to_create_pod_ptr to_create_pod
       (* TODO: specify that created_pod shares some contents with to_create_pod *)
   }}}.
 Proof.
+  wp_start as "H". iNamed "H".
 Admitted.
 
 Lemma wp_FormatInt (i: w64) (base: w64):
